safechecker/theories/PCUICTypeChecker.v
@@ -191,19 +191,17 @@ Section Typecheck.
   (* We get stack overflow on Qed after Equations definitions when this is transparent *)
   Opaque reduce_stack_full.
 
-  Notation hnf := (hnf HΣ).
-
-  
+  Notation hnf := (hnf (_Σ := Σ)).  
 
   (* replaces convert and convert_leq*)
   Equations convert (le : conv_pb) Γ t u
           (ht : welltyped gΣ Γ t) (hu : welltyped gΣ Γ u)
     : typing_result_comp (∥ gΣ ;;; Γ ⊢ t ≤[le] u ∥) :=
     convert le Γ t u ht hu
-      with inspect (eqb_termp Σ G le t u) := {
+      with inspect (eqb_termp_napp_gen le (wf_env_eq Σ) (wf_env_leq Σ) (wf_env_compare_global_instance Σ) 0 t u) := {
         | @exist true He := ret _ ; 
         | @exist false He with
-          inspect (isconv_term _ Σ G HG Γ le t ht u hu) := {
+          inspect (isconv_term Γ le t ht u hu) := {
           | @exist ConvSuccess Hc := ret _ ;
           | @exist (ConvError e) Hc :=
             let t' := hnf Γ t ht in
@@ -211,10 +209,12 @@ Section Typecheck.
             raise (NotCumulSmaller false G Γ t u t' u' e)
       }}.
   Next Obligation.
+    rewrite <- wf_env_eq_correct, <- wf_env_leq_correct, <- wf_env_compare_global_instance_correct in He. 
     symmetry in He; eapply eqb_termp_napp_spec in He ; tea.
-    all: sq.
-    2-3: now destruct HΣ.
+    all: pose heΣ as heΣ; sq.
+    2-3: now destruct heΣ.
     constructor ; auto ; fvs.
+    apply HG. 
   Qed.
   Next Obligation.
     now symmetry in Hc; apply isconv_term_sound in Hc.
@@ -234,17 +234,17 @@ Section Typecheck.
     end.
 
   Section InferAux.
-    Variable (infer : forall Γ (HΓ : ∥ wf_local Σ Γ ∥) (t : term),
-                 typing_result_comp ({ A : term & ∥ Σ ;;; Γ |- t ▹ A ∥ })).
+    Variable (infer : forall Γ (HΓ : ∥ wf_local gΣ Γ ∥) (t : term),
+                 typing_result_comp ({ A : term & ∥ gΣ ;;; Γ |- t ▹ A ∥ })).
 
-    Equations infer_type Γ (HΓ : ∥ wf_local Σ Γ ∥) t
-      : typing_result_comp ({u : Universe.t & ∥ Σ ;;; Γ |- t ▹□ u ∥}) :=
+    Equations infer_type Γ (HΓ : ∥ wf_local gΣ Γ ∥) t
+      : typing_result_comp ({u : Universe.t & ∥ gΣ ;;; Γ |- t ▹□ u ∥}) :=
       infer_type Γ HΓ t :=
         tx <- infer Γ HΓ t ;;
-        s <- reduce_to_sort HΣ Γ tx.π1 _ ;;
+        s <- reduce_to_sort (_Σ := Σ) Γ tx.π1 _ ;;
         ret (s.π1;_).
     Next Obligation.
-      sq.
+      pose HΣ. sq.
       eapply validity_wf ; auto.
       sq.
       now eapply infering_typing.
@@ -255,7 +255,7 @@ Section Typecheck.
       now apply closed_red_red.
     Defined.
     Next Obligation.
-      sq.
+      pose HΣ. sq.
       eapply absurd.
       eapply infering_sort_infering in X0; eauto.
     Qed.
@@ -267,40 +267,40 @@ Section Typecheck.
       now sq.
     Qed.
     
-    Equations infer_isType Γ (HΓ : ∥wf_local Σ Γ ∥) T : typing_result_comp (∥ isType Σ Γ T ∥) :=
+    Equations infer_isType Γ (HΓ : ∥wf_local gΣ Γ ∥) T : typing_result_comp (∥ isType gΣ Γ T ∥) :=
       infer_isType Γ HΓ T :=
         infer_type Γ HΓ T ;;
         ret _. 
     Next Obligation.
-      sq.
+      pose HΣ. sq.
       now eapply infering_sort_isType.
     Defined.
     Next Obligation.
-      sq.
+      pose HΣ. sq.
       apply absurd.
       eapply isType_infering_sort in H as [u ?].
       now exists u.
     Qed.
 
-    Equations bdcheck Γ (HΓ : ∥wf_local Σ Γ ∥) t A (hA : ∥ isType Σ Γ A ∥)
-      : typing_result_comp (∥ Σ ;;; Γ |- t ◃ A ∥) :=
+    Equations bdcheck Γ (HΓ : ∥wf_local gΣ Γ ∥) t A (hA : ∥ isType gΣ Γ A ∥)
+      : typing_result_comp (∥ gΣ ;;; Γ |- t ◃ A ∥) :=
       bdcheck Γ HΓ t A hA :=
         A' <- infer Γ HΓ t ;;
         convert Cumul Γ A'.π1 A _ _ ;;
         ret _.
     Next Obligation.
-    sq.
+    pose HΣ. sq.
     eapply validity_wf; auto.
     sq. now eapply infering_typing.
     Qed.
     Next Obligation. destruct hA; now apply wat_welltyped. Qed.
     Next Obligation.
-      sq.
+      pose HΣ; sq.
       econstructor ; tea.
       now apply equality_forget_cumul.
     Qed.
     Next Obligation.
-      sq.
+      pose HΣ. sq.
       apply absurd.
       sq.
       now eapply infering_checking ; fvs.
@@ -331,13 +331,13 @@ Section Typecheck.
       eapply type_reduction; eauto. exact r.
     Qed. *)
 
-    Lemma sq_wfl_nil : ∥ wf_local Σ [] ∥.
+    Lemma sq_wfl_nil : ∥ wf_local gΣ [] ∥.
     Proof.
      repeat constructor.
     Qed.
 
 
-    Equations check_context Γ : typing_result_comp (∥ wf_local Σ Γ ∥)
+    Equations check_context Γ : typing_result_comp (∥ wf_local gΣ Γ ∥)
     := 
       check_context [] := ret _ ;
       check_context ({| decl_body := None; decl_type := A |} :: Γ) :=
@@ -350,12 +350,12 @@ Section Typecheck.
         bdcheck Γ HΓ t A _  ;;
         ret _.
     Next Obligation.
-      sq.
+      pose HΣ. sq.
       econstructor ; tea.
       now eapply checking_typing.
     Qed.
     Next Obligation.
-    sq. eapply absurd. sq.
+    pose HΣ. sq. eapply absurd. sq.
     inversion H ; subst.
     now eapply typing_checking.
     Qed.
@@ -368,12 +368,12 @@ Section Typecheck.
       now inversion H.
     Qed.
     Next Obligation.
-      sq. econstructor; tas.
+      pose HΣ. sq. econstructor; tas.
       eexists.
       now eapply infering_sort_typing.
     Qed.
     Next Obligation.
-      sq. eapply absurd.
+      pose HΣ. sq. eapply absurd.
       inversion H ; subst.
       eapply isType_infering_sort in X0 as [] ; tea.
       eexists. now sq.
@@ -383,13 +383,13 @@ Section Typecheck.
       now inversion H.
     Qed.
  
-    Lemma sq_wf_local_app {Γ Δ} : ∥ wf_local Σ Γ ∥ -> ∥ wf_local_rel Σ Γ Δ ∥ -> ∥ wf_local Σ (Γ ,,, Δ) ∥.
+    Lemma sq_wf_local_app {Γ Δ} : ∥ wf_local gΣ Γ ∥ -> ∥ wf_local_rel gΣ Γ Δ ∥ -> ∥ wf_local gΣ (Γ ,,, Δ) ∥.
     Proof.
       intros. sq. now apply wf_local_app.
     Qed.
 
-    Equations check_context_rel Γ (wfΓ : ∥ wf_local Σ Γ ∥) (Δ : context) :
-      typing_result_comp (∥ wf_local_rel Σ Γ Δ ∥) :=
+    Equations check_context_rel Γ (wfΓ : ∥ wf_local gΣ Γ ∥) (Δ : context) :
+      typing_result_comp (∥ wf_local_rel gΣ Γ Δ ∥) :=
 
       check_context_rel Γ wfΓ [] := ret _ ;
 
@@ -407,11 +407,11 @@ Section Typecheck.
       sq. now constructor.
     Qed.
     Next Obligation.
-      sq. constructor ; auto.
+      pose HΣ. sq. constructor ; auto.
       eapply checking_typing ; pcuic.
     Qed.
     Next Obligation.
-      sq. apply absurd. sq.
+      pose HΣ. sq. apply absurd. sq.
       inversion H ; subst ; cbn in *.
       now eapply typing_checking.
     Qed.
@@ -439,8 +439,8 @@ Section Typecheck.
     Qed.
 
     Equations check_equality_decl (le : conv_pb) Γ d d'
-      (wtd : wt_decl Σ Γ d) (wtd' : wt_decl Σ Γ d')
-      : typing_result_comp (∥ equality_open_decls le Σ Γ d d' ∥) :=
+      (wtd : wt_decl gΣ Γ d) (wtd' : wt_decl gΣ Γ d')
+      : typing_result_comp (∥ equality_open_decls le gΣ Γ d d' ∥) :=
       check_equality_decl le Γ
         {| decl_name := na; decl_body := Some b; decl_type := ty |}
         {| decl_name := na'; decl_body := Some b'; decl_type := ty' |}
@@ -526,45 +526,45 @@ Section Typecheck.
     Qed.
 
     Lemma cumul_decls_irrel_sec Γ Γ' d d' :
-      cumul_decls Σ Γ Γ d d' ->
-      cumul_decls Σ Γ Γ' d d'.
+      cumul_decls gΣ Γ Γ d d' ->
+      cumul_decls gΣ Γ Γ' d d'.
     Proof.
       intros cum; depelim cum; intros; constructor; auto.
     Qed.
     
     Lemma conv_decls_irrel_sec Γ Γ' d d' :
-      conv_decls Σ Γ Γ d d' ->
-      conv_decls Σ Γ Γ' d d'.
+      conv_decls gΣ Γ Γ d d' ->
+      conv_decls gΣ Γ Γ' d d'.
     Proof.
       intros cum; depelim cum; intros; constructor; auto.
     Qed.
 
     Lemma inv_wf_local Γ d :
-      wf_local Σ (Γ ,, d) ->
-      wf_local Σ Γ * wt_decl Σ Γ d.
+      wf_local gΣ (Γ ,, d) ->
+      wf_local gΣ Γ * wt_decl gΣ Γ d.
     Proof.
       intros wfd; depelim wfd; split; simpl; pcuic.
       now exists t.
     Qed.
 
-    Lemma cumul_ctx_rel_cons {Γ Δ Δ' d d'} (c : cumul_ctx_rel Σ Γ Δ Δ') 
-      (p : cumul_decls Σ (Γ,,, Δ) (Γ ,,, Δ') d d') : 
-      cumul_ctx_rel Σ Γ (Δ ,, d) (Δ' ,, d').
+    Lemma cumul_ctx_rel_cons {Γ Δ Δ' d d'} (c : cumul_ctx_rel gΣ Γ Δ Δ') 
+      (p : cumul_decls gΣ (Γ,,, Δ) (Γ ,,, Δ') d d') : 
+      cumul_ctx_rel gΣ Γ (Δ ,, d) (Δ' ,, d').
     Proof.
       destruct d as [na [b|] ty], d' as [na' [b'|] ty']; try constructor; auto.
     Qed.
     
-    Lemma context_equality_rel_cons {le Γ Δ Δ' d d'} (c : context_equality_rel le Σ Γ Δ Δ') 
-      (p : equality_open_decls le Σ (Γ,,, Δ) d d') : 
-      context_equality_rel le Σ Γ (Δ ,, d) (Δ' ,, d').
+    Lemma context_equality_rel_cons {le Γ Δ Δ' d d'} (c : context_equality_rel le gΣ Γ Δ Δ') 
+      (p : equality_open_decls le gΣ (Γ,,, Δ) d d') : 
+      context_equality_rel le gΣ Γ (Δ ,, d) (Δ' ,, d').
     Proof.
       destruct c. split; auto.
       destruct d as [na [b|] ty], d' as [na' [b'|] ty']; try constructor; auto.
     Qed.
 
     Equations check_equality_ctx (le : conv_pb) Γ Δ Δ'
-      (wfΔ : ∥ wf_local Σ (Γ ,,, Δ) ∥) (wfΔ' : ∥ wf_local Σ (Γ ,,, Δ') ∥) : 
-      typing_result_comp (∥ context_equality_rel le Σ Γ Δ Δ' ∥) :=
+      (wfΔ : ∥ wf_local gΣ (Γ ,,, Δ) ∥) (wfΔ' : ∥ wf_local gΣ (Γ ,,, Δ') ∥) : 
+      typing_result_comp (∥ context_equality_rel le gΣ Γ Δ Δ' ∥) :=
 
       check_equality_ctx le Γ [] [] _ _ := ret _ ;
       
@@ -577,7 +577,7 @@ Section Typecheck.
         raise (Msg "While checking cumulativity of contexts: contexts do not have the same length").
       
       Next Obligation.
-        sq.
+        pose HΣ. sq.
         split.
         * fvs.
         * constructor.
@@ -601,7 +601,7 @@ Section Typecheck.
         destruct l; split; eexists; eauto.
       Qed.
       Next Obligation.
-        sq.
+        pose HΣ. sq.
         simpl in *.
         eapply inv_wf_local in wfΔ as [wfΔ wfd].
         eapply inv_wf_local in wfΔ' as [wfΔ' wfd'].
@@ -618,12 +618,12 @@ Section Typecheck.
         now apply context_equality_rel_cons.
       Qed.
       Next Obligation.
-        sq. apply absurd. sq.
+        pose HΣ. sq. apply absurd. sq.
         eapply context_equality_rel_app in H.
         now depelim H.
       Qed.
       Next Obligation.
-        sq. apply absurd. sq.
+        pose HΣ. sq. apply absurd. sq.
         eapply context_equality_rel_app in H.
         depelim H.
         now apply context_equality_rel_app.
@@ -674,8 +674,8 @@ Section Typecheck.
     Qed.
 
 
-    Equations check_inst Γ (wfΓ : ∥ wf_local Σ Γ ∥) Δ (wfΔ : ∥ wf_local_rel Σ Γ (List.rev Δ) ∥) (HΔ : assumption_context Δ) ts : 
-      typing_result_comp (∥ ctx_inst Σ Γ ts Δ ∥) by struct ts :=
+    Equations check_inst Γ (wfΓ : ∥ wf_local gΣ Γ ∥) Δ (wfΔ : ∥ wf_local_rel gΣ Γ (List.rev Δ) ∥) (HΔ : assumption_context Δ) ts : 
+      typing_result_comp (∥ ctx_inst gΣ Γ ts Δ ∥) by struct ts :=
     check_inst Γ _ [] _ _ [] := ret _ ;
     check_inst Γ wfΓ
       ({|decl_name := na ; decl_body := Some ; decl_type := T|} :: Δ)
@@ -707,7 +707,7 @@ Section Typecheck.
       now depelim wt.
     Qed.
     Next Obligation.
-      sq.
+      pose HΣ. sq.
       rewrite -subst_context_rev_subst_telescope.
       eapply substitution_wf_local_rel ; tea.
       constructor.
@@ -721,7 +721,7 @@ Section Typecheck.
       sq. depelim HΔ. now apply assumption_context_subst_telescope.
     Qed.
     Next Obligation.
-      sq.
+      pose HΣ. sq.
       constructor ; tea.
       apply checking_typing ; auto.
       eapply All_local_env_app_l in wfΔ.
@@ -732,13 +732,13 @@ Section Typecheck.
       now depelim H.
     Qed.
     Next Obligation.
-      sq. apply absurd. sq.
+      pose HΣ. sq. apply absurd. sq.
       apply typing_checking.
       now depelim H.
     Qed.
     
-    Equations check_equality_terms Γ ts ts' (wts : ∥ All (welltyped Σ Γ) ts ∥) (wts' : ∥ All (welltyped Σ Γ) ts' ∥) : 
-      typing_result_comp (∥ equality_terms Σ Γ ts ts' ∥) :=
+    Equations check_equality_terms Γ ts ts' (wts : ∥ All (welltyped gΣ Γ) ts ∥) (wts' : ∥ All (welltyped gΣ Γ) ts' ∥) : 
+      typing_result_comp (∥ equality_terms gΣ Γ ts ts' ∥) :=
     check_equality_terms Γ [] [] _ _ := ret _ ;
     check_equality_terms Γ (t :: ts) (t' :: ts') wts wts' :=
       convt <- convert Conv Γ t t' _ _ ;;
@@ -779,9 +779,9 @@ Section Typecheck.
 
   Equations lookup_ind_decl ind
     : typing_result_comp
-        ({decl & {body & declared_inductive (fst Σ) ind decl body}}) :=
+        ({decl & {body & declared_inductive (fst gΣ) ind decl body}}) :=
   lookup_ind_decl ind with
-    inspect (lookup_env (fst Σ) ind.(inductive_mind)) := {
+    inspect (wf_env_lookup Σ ind.(inductive_mind)) := {
       | @exist (Some (InductiveDecl decl)) _ 
           with inspect (nth_error decl.(ind_bodies) ind.(inductive_ind)) := {
             | @exist (Some body) _ => ret _ ;
@@ -791,11 +791,12 @@ Section Typecheck.
       }.
   Next Obligation.
     depelim X1.
-    depelim H.
+    depelim H. rewrite <- wf_env_lookup_correct in e0. 
+    rewrite <- e0 in H.   
     congruence.
   Qed.
   Next Obligation.
-    exists decl, body.
+    exists decl, body. rewrite <- wf_env_lookup_correct in e.  
     now split.
   Defined.
 
@@ -814,20 +815,21 @@ Section Typecheck.
   Qed.   
 
   Lemma subst_global_uctx_invariants inst cstrs (u : Instance.t) :
-    global_uctx_invariants (global_ext_uctx (Σ.1,Polymorphic_ctx (inst, cstrs))) ->
-    Forall (fun l => LevelSet.mem l (global_ext_levels Σ)) u ->
-    global_uctx_invariants ((global_ext_uctx Σ).1,subst_instance_cstrs u cstrs).
+    global_uctx_invariants (global_ext_uctx (gΣ.1,Polymorphic_ctx (inst, cstrs))) ->
+    Forall (fun l => LevelSet.mem l (global_ext_levels gΣ)) u ->
+    global_uctx_invariants ((global_ext_uctx gΣ).1,subst_instance_cstrs u cstrs).
   Proof.
     sq.
     intros [_ Hcs] Hu. split.
     - apply LevelSet.union_spec. right. apply global_levels_Set.
-    - pose proof Σ as [Σ' φ]. pose proof HΣ as [HΣ' Hφ].
+    - pose proof gΣ as [Σ' φ]. pose proof heΣ as [[HΣ' Hφ]].
+      pose proof heΣ as [heΣ].
       rewrite /uctx_invariants /= in Hcs |- *.
       intros [[l ct] l'] Hctr.
       rewrite /subst_instance_cstrs /= in Hctr.
       rewrite ConstraintSetProp.fold_spec_right in Hctr.
       set cstrs' := (List.rev (CS.elements cstrs)) in Hctr.
-      set Σ'' := (Σ.1,Polymorphic_ctx (inst, cstrs)) in Hcs.
+      set Σ'' := (gΣ.1,Polymorphic_ctx (inst, cstrs)) in Hcs.
       assert ((exists ct' l'', SetoidList.InA eq (l,ct',l'') cstrs') ->
         declared l (global_ext_levels Σ'')) as Hcs'.
       {
@@ -891,9 +893,9 @@ Section Typecheck.
              now eapply LevelSetFact.mem_1, wf_ext_global_uctx_invariants.
   Qed.
 
-  Equations check_consistent_instance uctx (wfg : ∥ global_uctx_invariants (global_ext_uctx (Σ.1, uctx)) ∥) 
+  Equations check_consistent_instance uctx (wfg : ∥ global_uctx_invariants (global_ext_uctx (gΣ.1, uctx)) ∥) 
     u
-    : typing_result_comp (consistent_instance_ext Σ uctx u) :=
+    : typing_result_comp (consistent_instance_ext gΣ uctx u) :=
   check_consistent_instance (Monomorphic_ctx _) wfg u 
     with (Nat.eq_dec #|u| 0) := {
       | left _ := ret _ ;
@@ -913,19 +915,20 @@ Section Typecheck.
     repeat split.
     - symmetry in e2.
       eapply forallb_All in e2. eapply All_forallb'; tea.
-      clear -cf HG. intros x; simpl. now apply is_graph_of_uctx_levels.
+      clear -cf. pose HG. intros x; simpl. now apply is_graph_of_uctx_levels. 
     - now rewrite mapi_length in e1.
     - eapply check_constraints_spec ; eauto.
-      all: now sq ; destruct HΣ.
+      all: pose heΣ as heΣ; sq; destruct heΣ; eauto.
+      apply HG. 
   Qed.
   Next Obligation.
-    pose proof HΣ as [HΣ'].
+    pose proof heΣ as [heΣ'].
     destruct wfg as [wfg].
     suff: (@check_constraints cf G (subst_instance_cstrs u cstrs)) by congruence.
     eapply check_constraints_complete. 
     - now eapply wf_ext_global_uctx_invariants.
     - now apply wf_ext_consistent.
-    - auto.
+    - apply HG.
     - eapply nor.
     - eapply (subst_global_uctx_invariants inst) => //.
       now eapply forallb_Forall in H.
@@ -933,7 +936,7 @@ Section Typecheck.
   Qed.
   Next Obligation.
     sq.
-    clear -e2 H HG.
+    clear -e2 H. pose HG.
     (* todo: should be a lemma? *)
     induction u.
     1: now cbn in * ; congruence.
@@ -950,20 +953,24 @@ Section Typecheck.
     now rewrite mapi_length in e1.
   Qed.
   Next Obligation.
-    inversion X1.
+    inversion X1. rewrite <- wf_env_lookup_correct in e1.
+    unfold declared_inductive, declared_minductive in H.
+    rewrite <- e1 in H.   
     congruence.
   Qed.
   Next Obligation.
-    inversion X1.
+    inversion X1. rewrite <- wf_env_lookup_correct in e0.
+    unfold declared_inductive, declared_minductive in H.
+    rewrite <- e0 in H.   
     congruence.
   Qed.
 
   (* Obligation Tactic := Program.Tactics.program_simplify ; eauto 2. *)
   
   Equations check_is_allowed_elimination
-    (u : Universe.t) (wfu : wf_universe Σ u)
+    (u : Universe.t) (wfu : wf_universe gΣ u)
     (al : allowed_eliminations) :
-    typing_result_comp (is_allowed_elimination Σ u al) :=
+    typing_result_comp (is_allowed_elimination gΣ u al) :=
 
   check_is_allowed_elimination u wfu IntoSProp
     with inspect (Universe.is_sprop u) := {
@@ -976,7 +983,7 @@ Section Typecheck.
       | @exist false _ := raise (Msg "Cannot eliminate over this sort")
     };
   check_is_allowed_elimination u wfu IntoSetPropSProp 
-    with inspect (is_propositional u || check_eqb_universe G u Universe.type0) := {
+    with inspect (is_propositional u || wf_env_eq Σ u Universe.type0) := {
       | @exist true _ := ret _ ;
       | @exist false _ := raise (Msg "Cannot eliminate over this sort")
     } ;
@@ -990,8 +997,8 @@ Section Typecheck.
     now rewrite e.
   Qed.
   Next Obligation.
-    sq.
-    apply wf_ext_consistent in HΣ as [v Hv].
+    pose heΣ as heΣ; sq.
+    apply wf_ext_consistent in heΣ as [v Hv].
     rewrite /is_allowed_elimination /is_allowed_elimination0 nor_check_univs in H.
     specialize (H v Hv).
     destruct u => //=.
@@ -1008,14 +1015,14 @@ Section Typecheck.
       + discriminate.
   Qed.
   Next Obligation.
-    sq.
-    apply wf_ext_consistent in HΣ as [v Hv].
+    pose heΣ as heΣ; sq.
+    apply wf_ext_consistent in heΣ as [v Hv].
     rewrite /is_allowed_elimination /is_allowed_elimination0 nor_check_univs in H.
     specialize (H v Hv).
     destruct u => //=.
   Qed.
   Next Obligation.
-    sq.
+    pose heΣ as heΣ;  sq.
     rewrite /is_allowed_elimination /is_allowed_elimination0 nor_check_univs.
     intros val sat.
     unfold is_propositional in *.
@@ -1023,8 +1030,10 @@ Section Typecheck.
     - apply is_prop_val with (v := val) in prop; rewrite prop; auto.
     - destruct Universe.is_sprop eqn:sprop.
       + apply is_sprop_val with (v := val) in sprop; rewrite sprop; auto.
-      + destruct check_eqb_universe eqn:check; [|discriminate].
-        eapply check_eqb_universe_spec' in check; eauto.
+      + rewrite <- wf_env_eq_correct in e. 
+        destruct check_eqb_universe eqn:check; [|discriminate].
+        pose HG. 
+        eapply check_eqb_universe_spec' in check; eauto. 
         * unfold eq_universe, eq_universe0 in check.
           rewrite nor_check_univs in check.
           specialize (check val sat).
@@ -1033,14 +1042,15 @@ Section Typecheck.
         * now eapply global_ext_uctx_consistent.
   Qed.
   Next Obligation.
-    sq.
-    move: (HΣ) => /wf_ext_consistent [v Hv].
+    pose heΣ as heΣ. sq.
+    move: (heΣ) => /wf_ext_consistent [v Hv].
     rewrite /is_allowed_elimination /is_allowed_elimination0 nor_check_univs in H.
-    destruct u => //=.
+    destruct u => //=. pose HG. 
     unshelve epose proof (eq_universeP _ _ _ _ _ n Universe.type0 _ _) as e'; tea.
-    1-2: now sq ; destruct HΣ.
+    1-2: now sq ; destruct heΣ.
     1: move => l /UnivExprSet.singleton_spec -> ;
       now apply LevelSetFact.union_3, global_levels_Set.
+    rewrite <- wf_env_eq_correct in e0. 
     move: e0 => /= /ssrfun.esym /(elimF e') ne.
     apply ne.
     rewrite /eq_universe /eq_universe0 nor_check_univs.
@@ -1057,39 +1067,39 @@ Section Typecheck.
     (∥ All2i (fun i cdecl br =>
       let brctxty := case_branch_type ci.(ci_ind) mdecl idecl p br ptm i cdecl in
       eq_context_upto_names br.(bcontext) (cstr_branch_context ci mdecl cdecl) ×
-        Σ ;;; Γ ,,, brctxty.1 |- br.(bbody) ◃ brctxty.2)
+        gΣ ;;; Γ ,,, brctxty.1 |- br.(bbody) ◃ brctxty.2)
       n ctors brs ∥).
 
   Section check_brs.
-    Context (infer : forall (Γ : context) (HΓ : ∥ wf_local Σ Γ ∥) (t : term), typing_result_comp ({ A : term & ∥ Σ ;;; Γ |- t ▹ A ∥ }))
-     (Γ : context) (wfΓ : ∥ wf_local Σ Γ ∥) (ps : Universe.t)
+    Context (infer : forall (Γ : context) (HΓ : ∥ wf_local gΣ Γ ∥) (t : term), typing_result_comp ({ A : term & ∥ gΣ ;;; Γ |- t ▹ A ∥ }))
+     (Γ : context) (wfΓ : ∥ wf_local gΣ Γ ∥) (ps : Universe.t)
      (ci : case_info) (mdecl : mutual_inductive_body)
      (idecl : one_inductive_body) (p : predicate term) (args : list term).
      
-    Context (isdecl : declared_inductive Σ ci mdecl idecl).
-    Context (hty : ∥ isType Σ Γ (mkApps (tInd ci (puinst p)) (pparams p ++ args)) ∥).
+    Context (isdecl : declared_inductive gΣ ci mdecl idecl).
+    Context (hty : ∥ isType gΣ Γ (mkApps (tInd ci (puinst p)) (pparams p ++ args)) ∥).
     Context (wfp : wf_predicate mdecl idecl p).
     Context (predctx := case_predicate_context ci mdecl idecl p).
-    Context (wfpret : ∥ Σ;;; Γ,,, predctx |- preturn p ▹□ ps ∥).
+    Context (wfpret : ∥ gΣ;;; Γ,,, predctx |- preturn p ▹□ ps ∥).
     Context (ptm := it_mkLambda_or_LetIn predctx (preturn p)).
     Context (hpctx : ∥ eq_context_upto_names (pcontext p)
           (ind_predicate_context ci mdecl idecl) ∥).
              
     Lemma branch_helper n cdecl ctors br
-      (isdecl' : ∥ Alli (fun i cdecl => declared_constructor Σ (ci, i) mdecl idecl cdecl) n (cdecl :: ctors) ∥) : 
+      (isdecl' : ∥ Alli (fun i cdecl => declared_constructor gΣ (ci, i) mdecl idecl cdecl) n (cdecl :: ctors) ∥) : 
       ∥ eq_context_gen eq eq (bcontext br) (cstr_branch_context ci mdecl cdecl) ∥ ->
       ∥ wf_branch cdecl br ×
       let brctxty := case_branch_type ci.(ci_ind) mdecl idecl p br ptm n cdecl in
-      wf_local Σ (Γ,,, brctxty.1) × Σ;;; Γ,,, brctxty.1 |- brctxty.2 ◃ tSort ps ∥.
+      wf_local gΣ (Γ,,, brctxty.1) × gΣ;;; Γ,,, brctxty.1 |- brctxty.2 ◃ tSort ps ∥.
     Proof.
-      intros; sq.
+      intros; pose HΣ; sq.
       depelim isdecl'.
       have wfbr : wf_branch cdecl br.
       { do 2 red.
         unfold cstr_branch_context, expand_lets_ctx, expand_lets_k_ctx in H.
         move/eq_context_gen_binder_annot: H.
         now do 3 move/eq_annots_fold. }
-      assert (wfpret' : Σ ;;; Γ ,,, predctx |- preturn p : tSort ps).
+      assert (wfpret' : gΣ ;;; Γ ,,, predctx |- preturn p : tSort ps).
         { eapply infering_sort_typing ; eauto.
           now eapply wf_case_predicate_context. }
       destruct (wf_case_branch_type ps args isdecl hty wfp wfpret' hpctx _ _ _ d wfbr).
@@ -1101,7 +1111,7 @@ Section Typecheck.
 
     Equations check_branches (n : nat) (ctors : list constructor_body)
       (brs : list (branch term)) 
-      (isdecl : ∥ Alli (fun i cdecl => declared_constructor Σ (ci, i) mdecl idecl cdecl) n ctors ∥)
+      (isdecl : ∥ Alli (fun i cdecl => declared_constructor gΣ (ci, i) mdecl idecl cdecl) n ctors ∥)
       : typing_result_comp (wt_brs Γ ci mdecl idecl p ptm ctors brs n) by struct brs := 
 
       check_branches n [] [] i := ret _ ;
@@ -1135,7 +1145,7 @@ Section Typecheck.
     Defined.
     Next Obligation.
       eapply branch_helper in i; tea.
-      sq. 
+      pose HΣ; sq. 
       destruct i as [? []].
       exists ps.
       apply checking_typing ; eauto.
@@ -1196,11 +1206,11 @@ Section Typecheck.
   Qed.
 
   Section check_mfix.
-  Context (infer : forall (Γ : context) (HΓ : ∥ wf_local Σ Γ ∥) (t : term), typing_result_comp ({ A : term & ∥ Σ ;;; Γ |- t ▹ A ∥ }))
-     (Γ : context) (wfΓ : ∥ wf_local Σ Γ ∥).
+  Context (infer : forall (Γ : context) (HΓ : ∥ wf_local gΣ Γ ∥) (t : term), typing_result_comp ({ A : term & ∥ gΣ ;;; Γ |- t ▹ A ∥ }))
+     (Γ : context) (wfΓ : ∥ wf_local gΣ Γ ∥).
 
   Equations check_mfix_types (mfix : mfixpoint term)
-  : typing_result_comp (∥ All (fun x => isType Σ Γ (dtype x)) mfix ∥) :=
+  : typing_result_comp (∥ All (fun x => isType gΣ Γ (dtype x)) mfix ∥) :=
     check_mfix_types [] := Checked_comp (sq All_nil) ;
     (* (* probably not tail recursive but needed so that next line terminates *)
       check_mfix_types mfix ;;
@@ -1211,7 +1221,7 @@ Section Typecheck.
       check_mfix_types mfix ;;
       ret _.
   Next Obligation.
-    sq.
+    pose HΣ; sq.
     constructor ; tea.
     exists s.
     now apply infering_sort_typing.
@@ -1221,7 +1231,7 @@ Section Typecheck.
     now depelim H.
   Qed.
   Next Obligation.
-    sq. apply absurd. sq.
+    pose HΣ; sq. apply absurd. sq.
     depelim H.
     apply isType_infering_sort in i as [u ?]; tea.
     exists u.
@@ -1230,11 +1240,11 @@ Section Typecheck.
   
   Equations check_mfix_bodies
     (mfix : mfixpoint term)
-    (wf_types : ∥ All (fun x => isType Σ Γ (dtype x)) mfix ∥)
+    (wf_types : ∥ All (fun x => isType gΣ Γ (dtype x)) mfix ∥)
     (Δ : context)
-    (wfΔ : ∥ wf_local Σ (Γ,,,Δ) ∥)
+    (wfΔ : ∥ wf_local gΣ (Γ,,,Δ) ∥)
     : typing_result_comp (∥ All (fun d =>
-        Σ ;;; Γ ,,, Δ |-
+        gΣ ;;; Γ ,,, Δ |-
           dbody d ◃ (lift0 #|Δ|) (dtype d)) mfix∥) :=
 
     check_mfix_bodies [] _ _ _ := Checked_comp (sq All_nil) ;
@@ -1245,7 +1255,7 @@ Section Typecheck.
       ret _.
 
   Next Obligation.
-    sq.
+    pose HΣ; sq.
     apply isType_lift ; eauto.
     - len.
     - rewrite skipn_all_app.
@@ -1277,7 +1287,7 @@ Section Typecheck.
     now rewrite IHn skipn_S.
   Qed.
 
-  Lemma ctx_inst_wt Γ s Δ : ctx_inst Σ Γ s Δ -> All (welltyped Σ Γ) s.
+  Lemma ctx_inst_wt Γ s Δ : ctx_inst gΣ Γ s Δ -> All (welltyped gΣ Γ) s.
   Proof.
     induction 1; try constructor; auto.
     now exists t.
@@ -1286,8 +1296,8 @@ Section Typecheck.
   Local Notation check_eq_true b e :=
     (if b as b' return (typing_result_comp (is_true b')) then ret eq_refl else raise e).
 
-  Equations infer (Γ : context) (HΓ : ∥ wf_local Σ Γ ∥) (t : term)
-  : typing_result_comp ({ A : term & ∥ Σ ;;; Γ |- t ▹ A ∥ }) by struct t :=
+  Equations infer (Γ : context) (HΓ : ∥ wf_local gΣ Γ ∥) (t : term)
+  : typing_result_comp ({ A : term & ∥ gΣ ;;; Γ |- t ▹ A ∥ }) by struct t :=
 
   infer Γ HΓ (tRel n)
     with inspect (nth_error Γ n) := {
@@ -1299,7 +1309,7 @@ Section Typecheck.
 
   infer Γ HΓ (tEvar ev _) := raise (UnboundEvar ev) ;
 
-  infer Γ HΓ (tSort u) with inspect (wf_universeb Σ u) := {
+  infer Γ HΓ (tSort u) with inspect (wf_env_universe Σ u) := {
     | exist true _ := ret (tSort (Universe.super u);_) ;
     | exist false _ := raise (Msg ("Sort contains an undeclared level " ^ string_of_sort u))
   } ;
@@ -1322,12 +1332,12 @@ Section Typecheck.
 
   infer Γ HΓ (tApp t u) :=
     ty <- infer Γ HΓ t ;;
-    pi <- reduce_to_prod HΣ Γ ty.π1 _ ;;
+    pi <- reduce_to_prod (_Σ := Σ) Γ ty.π1 _ ;;
     bdcheck infer Γ HΓ u pi.π2.π1 _ ;;
     ret (subst10 u pi.π2.π2.π1; _) ;
 
   infer Γ HΓ (tConst cst u)
-    with inspect (lookup_env (fst Σ) cst) := {
+    with inspect (wf_env_lookup Σ cst) := {
     | exist (Some (ConstantDecl d)) HH =>
         check_consistent_instance d.(cst_universes) _ u ;;
         let ty := subst_instance u d.(cst_type) in
@@ -1353,7 +1363,7 @@ Section Typecheck.
 
   infer Γ HΓ (tCase ci p c brs) :=
     cty <- infer Γ HΓ c ;;
-    I <- reduce_to_ind HΣ Γ cty.π1 _ ;;
+    I <- reduce_to_ind (_Σ := Σ) Γ cty.π1 _ ;;
     (*let (ind';(u;(args;H))) := I in*)
     let ind' := I.π1 in let u := I.π2.π1 in let args := I.π2.π2.π1 in
     check_eq_true (eqb ci.(ci_ind) ind')
@@ -1372,14 +1382,14 @@ Section Typecheck.
     let chop_args := chop ci.(ci_npar) args
     in let params := chop_args.1 in let indices := chop_args.2 in
     cu <- check_consistent_instance (ind_universes mdecl) _ p.(puinst) ;;
-    check_eq_true (compare_global_instance Σ (check_eqb_universe G) (check_leqb_universe G) (IndRef ind') 
+    check_eq_true (wf_env_compare_global_instance Σ (check_leqb_universe G) (IndRef ind') 
       #|args| u p.(puinst))
       (Msg "invalid universe annotation on case, not larger than the discriminee's universes") ;;
     wt_params <- check_inst infer Γ HΓ (List.rev (smash_context [] (ind_params mdecl))@[p.(puinst)]) _ _ p.(pparams) ;;
     eq_params <- check_equality_terms Γ params p.(pparams) _ _ ;;
     let pctx := case_predicate_context ci.(ci_ind) mdecl idecl p in
     check_wfpctx_conv <- check_alpha_equality_ctx p.(pcontext) (ind_predicate_context ci mdecl idecl) ;;
-    let isty : ∥ isType Σ Γ (mkApps (tInd ci p.(puinst)) (p.(pparams) ++ indices)) ∥ := _ in
+    let isty : ∥ isType gΣ Γ (mkApps (tInd ci p.(puinst)) (p.(pparams) ++ indices)) ∥ := _ in
     let wfp : ∥ wf_predicate mdecl idecl p ∥ := _ in
     ps <- infer_type infer (Γ ,,, pctx) _ p.(preturn) ;;
     check_is_allowed_elimination ps.π1 _ (ind_kelim idecl);;
@@ -1395,7 +1405,7 @@ Section Typecheck.
         | exist None _ := raise (Msg "projection not found") ;
         | exist (Some pdecl) HH =>
             c_ty <- infer Γ HΓ c ;;
-            I <- reduce_to_ind HΣ Γ c_ty.π1 _ ;;
+            I <- reduce_to_ind (_Σ := Σ) Γ c_ty.π1 _ ;;
             (*let (ind';(u;(args;H))) := I in*)
             let ind' := I.π1 in let u := I.π2.π1 in let args := I.π2.π2.π1 in
             check_eq_true (eqb ind ind')
@@ -1412,8 +1422,9 @@ Section Typecheck.
     | exist (Some decl) Hnth :=
       wf_types <- check_mfix_types infer Γ HΓ mfix ;;
       wf_bodies <- check_mfix_bodies infer Γ HΓ mfix _ (fix_context mfix) _ ;;
-      guarded <- check_eq_true (fix_guard Σ Γ mfix) (Msg "Unguarded fixpoint") ;;
-      wffix <- check_eq_true (wf_fixpoint Σ.1 mfix) (Msg "Ill-formed fixpoint: not defined on a mutually inductive family") ;;
+    (* TODO use abstract check here *)
+      guarded <- check_eq_true (fix_guard gΣ Γ mfix) (Msg "Unguarded fixpoint") ;;
+      wffix <- check_eq_true (wf_fixpoint gΣ.1 mfix) (Msg "Ill-formed fixpoint: not defined on a mutually inductive family") ;;
       ret (dtype decl; _) };
 
   infer Γ HΓ (tCoFix mfix n)
@@ -1422,8 +1433,9 @@ Section Typecheck.
     | exist (Some decl) Hnth :=
       wf_types <- check_mfix_types infer Γ HΓ mfix ;;
       wf_bodies <- check_mfix_bodies infer Γ HΓ mfix _ (fix_context mfix) _ ;;
-      guarded <- check_eq_true (cofix_guard Σ Γ mfix) (Msg "Unguarded cofixpoint") ;;
-      wfcofix <- check_eq_true (wf_cofixpoint Σ.1 mfix) (Msg "Ill-formed cofixpoint: not producing values in a mutually coinductive family") ;;
+    (* TODO use abstract check here *)
+    guarded <- check_eq_true (cofix_guard gΣ Γ mfix) (Msg "Unguarded cofixpoint") ;;
+      wfcofix <- check_eq_true (wf_cofixpoint gΣ.1 mfix) (Msg "Ill-formed cofixpoint: not producing values in a mutually coinductive family") ;;
       ret (dtype decl; _)
     } ;
 
@@ -1438,19 +1450,19 @@ Section Typecheck.
   Next Obligation. intros; sq; now inversion X0. Qed.
   (* tSort *)
   Next Obligation.
-    symmetry in e.
+    symmetry in e. rewrite <- wf_env_universe_correct in e. 
     eapply (elimT wf_universe_reflect) in e.
     sq; econstructor; tas.
   Defined.
   Next Obligation.
     sq.
-    inversion X0 ; subst.
+    inversion X0 ; subst. rewrite <- wf_env_universe_correct in e0. 
     move: H0 e0 => /wf_universe_reflect -> //.
   Qed.
   (* tProd *)
   Next Obligation.
     (* intros Γ HΓ t na A B Heq_t [s ?];  *)
-    sq; econstructor ; tea.
+    pose HΣ; sq; econstructor ; tea.
     now eapply infering_sort_isType.
   Defined.
   Next Obligation.
@@ -1470,12 +1482,12 @@ Section Typecheck.
   (* tLambda *)
   Next Obligation.
     (* intros Γ HΓ t0 na A t Heq_t [s ?]; *)
-      sq; econstructor; tea.
+    pose HΣ; sq; econstructor; tea.
       now eapply infering_sort_isType.
   Defined.
   Next Obligation.
     (* intros Γ HΓ t0 na A t Heq_t [s ?] [B ?]; *)
-      sq; econstructor; eassumption.
+      pose HΣ; sq; econstructor; eassumption.
   Defined.
   Next Obligation.
     sq. apply absurd.
@@ -1489,11 +1501,11 @@ Section Typecheck.
   Qed.
   (* tLetIn *)
   Next Obligation.
-      sq. now econstructor ; eapply infering_sort_typing ; eauto.
+  pose HΣ; sq. now econstructor ; eapply infering_sort_typing ; eauto.
   Defined.
   Next Obligation.
     (* intros Γ HΓ t n b b_ty b' Heq_t [? ?] H0; *)
-    sq.
+    pose HΣ; sq.
     econstructor ; tea.
     2: apply checking_typing ; eauto.
     all: now eapply infering_sort_isType.
@@ -1518,13 +1530,13 @@ Section Typecheck.
   Qed.
   (* tApp *)
   Next Obligation.
-    sq.
+  pose HΣ; sq.
     eapply validity_wf ; eauto.
     sq.
     now apply infering_typing.
   Qed.
   Next Obligation.
-    cbn in *; sq.
+    cbn in *; pose HΣ as HΣ; sq.
     eapply infering_typing, type_reduction_closed, validity in X2.
     2-4: eauto.
     destruct X2 as [s HH].
@@ -1539,7 +1551,7 @@ Section Typecheck.
     now apply closed_red_red.
   Defined.
   Next Obligation.
-    sq. apply absurd. sq.
+  pose HΣ; sq. apply absurd. sq.
     inversion X0 ; subst.
     assert (is_open_term Γ A).
     {
@@ -1564,7 +1576,7 @@ Section Typecheck.
     now eapply red_equality.
   Qed.
   Next Obligation.
-    sq. apply absurd.
+  pose HΣ; sq. apply absurd.
     inversion X0 ; subst.
     eapply infering_prod_infering in X2 as (A'&B'&[]) ; eauto.
   Qed.
@@ -1576,35 +1588,36 @@ Section Typecheck.
   
   (* tConst *)
   Next Obligation.
-    sq. eapply global_uctx_invariants_ext.
-    symmetry in HH.
+    pose HΣ as HΣ; sq. eapply global_uctx_invariants_ext.
+    symmetry in HH. rewrite <- wf_env_lookup_correct in HH. 
     now apply (weaken_lookup_on_global_env' _ _ _ HΣ HH).
   Qed.
   Next Obligation.
-    sq; constructor; try assumption.
-    symmetry in HH.
+    pose HΣ; sq; constructor; try assumption.
+    symmetry in HH. rewrite <- wf_env_lookup_correct in HH. 
     etransitivity. eassumption. reflexivity.
   Defined.
   Next Obligation.
-    sq. apply absurd.
-    now inversion X0.
+    pose HΣ; sq. apply absurd. rewrite <- wf_env_lookup_correct in HH. 
+    inversion X0. unfold declared_constant in isdecl.
+    rewrite <- HH in isdecl. inversion isdecl. now subst.  
   Qed.
   Next Obligation.
     sq.
-    inversion X0 ; subst.
+    inversion X0 ; subst. rewrite <- wf_env_lookup_correct in e0.
     rewrite isdecl in e0.
     congruence.
   Qed.
   Next Obligation.
     sq.
-    inversion X0 ; subst.
+    inversion X0 ; subst. rewrite <- wf_env_lookup_correct in e0.
     rewrite isdecl in e0.
     congruence.
   Qed.
 
   (* tInd *)
   Next Obligation.
-    sq. eapply global_uctx_invariants_ext.
+    pose HΣ as HΣ. sq. eapply global_uctx_invariants_ext.
     eapply (weaken_lookup_on_global_env' _ _ _ HΣ (proj1 X0)).
   Qed.
   Next Obligation.
@@ -1624,7 +1637,7 @@ Section Typecheck.
 
   (* tConstruct *)
   Next Obligation.
-    sq. eapply global_uctx_invariants_ext.
+    pose HΣ as HΣ. sq. eapply global_uctx_invariants_ext.
     eapply (weaken_lookup_on_global_env' _ _ _ HΣ (proj1 decl)).
   Qed.
   Next Obligation.
@@ -1656,17 +1669,17 @@ Section Typecheck.
 
   (* tCase *)
   Next Obligation.
-    sq.
+    pose HΣ. sq.
     eapply infering_typing, validity in X as []; eauto.
     eexists; eauto using validity_wf.
   Defined.
   Next Obligation.
-    sq. eapply global_uctx_invariants_ext.
+    pose HΣ as HΣ. sq. eapply global_uctx_invariants_ext.
     eapply (weaken_lookup_on_global_env' _ _ _ HΣ (proj1 X0)).
   Qed.
   Next Obligation.
     rewrite List.rev_involutive.
-    sq.
+    pose HΣ. sq.
     eapply wf_rel_weak ; eauto.
     rewrite subst_instance_smash ; eapply wf_local_smash_context.
     now eapply on_minductive_wf_params.
@@ -1676,7 +1689,7 @@ Section Typecheck.
     apply assumption_context_subst_instance, smash_context_assumption_context; constructor.
   Qed.
   Next Obligation.
-    sq.
+    pose HΣ as HΣ. sq.
     apply eqb_eq in i. subst I.
     apply eqb_eq in i0.
     rewrite chop_firstn_skipn -i0 /=.
@@ -1694,7 +1707,7 @@ Section Typecheck.
     
   Next Obligation.
     (*todo: factor*)
-    sq.
+    pose heΣ as HΣ. sq.
     apply eqb_eq in i. subst I.
     eapply eqb_eq in i0.
     rewrite chop_firstn_skipn -i0 /=.
@@ -1707,7 +1720,7 @@ Section Typecheck.
     { eapply weaken_wf_local; eauto. eapply on_minductive_wf_params; eauto. }
     eexists; eapply isType_mkApps_Ind_smash; tea.
     rewrite subst_instance_app List.rev_app_distr smash_context_app_expand.
-    have wf_ctx : wf_local Σ
+    have wf_ctx : wf_local gΣ
       (Γ,,, smash_context [] (ind_params d)@[puinst p],,,
       expand_lets_ctx (ind_params d)@[puinst p]
        (smash_context [] (ind_indices X)@[puinst p])).
@@ -1747,9 +1760,11 @@ Section Typecheck.
       rewrite -(subst_context_smash_context _ _ []).
       rewrite -(spine_subst_inst_subst X3).
       rewrite - !smash_context_subst /= !subst_context_nil.
+      rewrite <- wf_env_compare_global_instance_correct in i1. 
       eapply compare_global_instance_sound in i1; pcuic.
       2: now destruct HΣ.
       eapply (inductive_cumulative_indices X0); tea.
+      apply HG. 
   Qed.
   
   Obligation Tactic := idtac.
@@ -1760,7 +1775,7 @@ Section Typecheck.
     destruct I as [ind' [u [args []]]].
     destruct d as [mdecl [idecl isdecl]].
     cbn in *.
-    sq.
+    pose HΣ. sq.
     apply eqb_eq in i. subst ind'.
     eapply eqb_eq in i0.
     eapply eq_context_gen_wf_predicate; tea.
@@ -1773,7 +1788,7 @@ Section Typecheck.
 
   Next Obligation.
     intros.
-    sq.
+    pose HΣ. sq.
     now eapply wf_case_predicate_context.
   Qed.
 
@@ -1781,7 +1796,7 @@ Section Typecheck.
     intros. simpl in *.
     clearbody isty wfp.
     destruct ps as [u' pty] ; cbn.
-    sq.
+    pose HΣ. sq.
     eapply isType_Sort_inv, validity, infering_sort_typing.
     3: eapply wf_case_predicate_context.
     all: eauto.
@@ -1818,7 +1833,7 @@ Section Typecheck.
     destruct d as [mdecl [idecl isdecl]].
     destruct ps as [ps ?].
     cbn in *.
-    sq.
+    pose heΣ as HΣ. sq.
     apply eqb_eq in i. subst ind'.
     eapply eqb_eq in i0.
     rewrite /indices /chop_args chop_firstn_skipn /=.
@@ -1841,8 +1856,9 @@ Section Typecheck.
       eapply ctx_inst_smash.
       now rewrite subst_instance_smash /= in wt_params.
       - now eapply negbTE.
-    - eapply compare_global_instance_sound ; tea.
-      now destruct HΣ.
+    - rewrite <- wf_env_compare_global_instance_correct in i1. 
+      eapply compare_global_instance_sound ; tea.
+      now destruct HΣ. apply HG. 
     - rewrite /params /chop_args chop_firstn_skipn /= in eq_params.
       eapply All2_impl ; tea.
       intros ? ? ?.
@@ -1868,7 +1884,7 @@ Section Typecheck.
     destruct d as [mdecl [idecl isdecl]].
     destruct ps as [ps ?].
     cbn in *.
-    intros. sq.
+    intros. pose heΣ as HΣ. sq.
     destruct X as [? [ty]].
     inversion ty ; subst.
     eapply declared_inductive_inj in isdecl as []; tea.
@@ -1891,7 +1907,7 @@ Section Typecheck.
     destruct d as [mdecl [idecl isdecl]].
     destruct ps as [ps ?].
     cbn in *.
-    intros. sq.
+    intros. pose heΣ as HΣ. sq.
     destruct X as [? [ty]].
     inversion ty ; subst.
     eapply declared_inductive_inj in isdecl as []; tea.
@@ -1941,7 +1957,7 @@ Section Typecheck.
     destruct I as [ind' [u [args []]]].
     destruct d as [mdecl [idecl isdecl]].
     cbn in *.
-    intros. sq.
+    intros. pose heΣ as HΣ. sq.
     destruct X as [? [ty]].
     inversion ty ; subst.
     eapply declared_inductive_inj in isdecl as []; tea.
@@ -1973,7 +1989,7 @@ Section Typecheck.
     destruct I as [ind' [u [args []]]].
     destruct d as [mdecl [idecl isdecl]].
     cbn in *.
-    intros. sq.
+    intros. pose heΣ as HΣ. sq.
     destruct X as [? [ty]].
     inversion ty ; subst.
     eapply declared_inductive_inj in isdecl as []; tea.
@@ -1998,11 +2014,13 @@ Section Typecheck.
     eapply declared_inductive_inj in isdecl as []; tea.
     subst.
     apply absurd.
-    unshelve eapply (compare_global_instance_complete _ _ _ _ _ _ Cumul) ; tea.
-    - sq.
+    rewrite <- wf_env_compare_global_instance_correct in absurd.
+    rewrite <- wf_env_compare_global_instance_correct. 
+    unshelve eapply (compare_global_instance_complete _ _ Cumul) ; tea.
+    - pose heΣ as HΣ. sq.
       apply/wf_universe_instanceP.
       rewrite -wf_universeb_instance_forall.
-      assert (tyu : isType Σ Γ (mkApps (tInd ind' u) args)).
+      assert (tyu : isType gΣ Γ (mkApps (tInd ind' u) args)).
       {
         eapply isType_red.
         2: exact c0.
@@ -2012,13 +2030,13 @@ Section Typecheck.
       rewrite wf_universes_mkApps in tyu.
       now move: tyu => /andP [].
 
-    - sq.
+    - pose heΣ as HΣ. sq.
       apply infering_typing, typing_wf_universes in ty ; auto.
       move: ty => /andP [].
       now rewrite {1}/wf_universes /= wf_universeb_instance_forall =>
         /andP [] /wf_universe_instanceP.
 
-    - sq.
+    - pose heΣ as HΣ. sq.
       eapply infering_ind_ind in X as [args'' []].
       2-3: now auto.
       2: now econstructor ; tea ; apply closed_red_red.
@@ -2092,7 +2110,7 @@ Section Typecheck.
     destruct X as [? [ty]].
     inversion ty ; subst.
     cbn in *.
-    sq.
+    pose heΣ as HΣ. sq.
     apply absurd.
     eapply infering_ind_ind in X as [? []].
     2-3: now auto.
@@ -2106,7 +2124,7 @@ Section Typecheck.
     destruct X as [? [ty]].
     inversion ty ; subst.
     cbn in *.
-    sq.
+    pose heΣ as HΣ. sq.
     apply absurd.
     inversion X ; subst.
     apply into_closed_red in X7.
@@ -2134,9 +2152,12 @@ Section Typecheck.
   Obligation Tactic := Program.Tactics.program_simplify ; eauto 2.
 
   (* tProj *)
-  Next Obligation. sq. eapply validity_wf ; eauto. sq. now eapply infering_typing. Defined.
+  Next Obligation. 
+    pose heΣ as HΣ. sq. eapply validity_wf ; eauto. sq. 
+    now eapply infering_typing. 
+  Defined.
   Next Obligation.
-    simpl in *; sq.
+    simpl in *; pose heΣ as HΣ. sq.
     pose proof (on_declared_inductive decl) as [onmib oni].
     eapply onProjections in oni.
     destruct ind_ctors as [|? []] eqn:hctors => //.
@@ -2180,7 +2201,7 @@ Section Typecheck.
     eapply Nat.eqb_refl.
   Qed.
   Next Obligation.
-    sq.
+  pose heΣ as HΣ. sq.
     apply absurd.
     apply/eqb_spec.
     cbn in *.
@@ -2194,7 +2215,7 @@ Section Typecheck.
   Qed.
   Next Obligation.
     cbn in *.
-    sq.
+    pose heΣ as HΣ. sq.
     apply absurd.
     inversion X0 ; subst.
     inversion X2 ; subst.
@@ -2234,9 +2255,9 @@ Section Typecheck.
   Qed.
 
   (* tFix *)
-  Next Obligation. sq. now eapply All_mfix_wf. Defined.
+  Next Obligation. pose heΣ as HΣ. sq. now eapply All_mfix_wf. Defined.
   Next Obligation.
-    sq.
+  pose heΣ as HΣ. sq.
     constructor; auto.
     eapply All_impl ; tea.
     intros.
@@ -2259,7 +2280,7 @@ Section Typecheck.
     now inversion X0 ; subst.
   Qed.
   Next Obligation.
-    sq.
+  pose heΣ as HΣ. sq.
     apply absurd.
     sq.
     inversion X0 ; subst.
@@ -2275,9 +2296,9 @@ Section Typecheck.
   Qed.
 
   (* tCoFix *)
-  Next Obligation. sq. now eapply All_mfix_wf. Defined.
+  Next Obligation. pose heΣ as HΣ. sq. now eapply All_mfix_wf. Defined.
   Next Obligation.
-    sq.
+  pose heΣ as HΣ. sq.
     constructor; auto.
     eapply All_impl ; tea.
     intros.
@@ -2300,7 +2321,7 @@ Section Typecheck.
     now inversion X0 ; subst.
   Qed.
   Next Obligation.
-    sq.
+  pose heΣ as HΣ. sq.
     apply absurd.
     sq.
     inversion X0 ; subst.
@@ -2334,24 +2355,24 @@ Section Typecheck.
 
   Definition check_isType := infer_isType infer.
 
-  Equations check Γ (HΓ : ∥ wf_local Σ Γ ∥) t A
-    : typing_result_comp (∥ Σ;;; Γ |- t : A ∥) :=
+  Equations check Γ (HΓ : ∥ wf_local gΣ Γ ∥) t A
+    : typing_result_comp (∥ gΣ;;; Γ |- t : A ∥) :=
     check Γ HΓ t A :=
       check_isType Γ HΓ A ;;
       bdcheck infer Γ HΓ t A _ ;;
       ret _.
   Next Obligation.
-    sq.
+  pose heΣ as HΣ. sq.
     now apply checking_typing.
   Qed.
   Next Obligation.
-    sq.
+  pose heΣ as HΣ. sq.
     apply absurd.
     sq.
     now apply typing_checking.
   Qed.
   Next Obligation.
-    sq.
+  pose heΣ as HΣ. sq.
     apply absurd.
     sq.
     now eapply validity.
